
% This LaTeX was auto-generated from MATLAB code.
% To make changes, update the MATLAB code and republish this document.

\documentclass[11pt]{article}
\usepackage[utf8]{inputenc}
\usepackage[T1]{fontenc}
\usepackage{amsthm}
\usepackage{enumitem}
\usepackage{amssymb}
\usepackage{amsmath}
\usepackage{amsfonts}
\usepackage[version=4]{mhchem}
\usepackage{stmaryrd}
\usepackage{mathrsfs}
\usepackage{bm}
\usepackage{graphicx}
\usepackage[export]{adjustbox}
\graphicspath{ {./images/} }
\usepackage{algorithm}
\usepackage{algorithmic}
\usepackage{makecell}  % 表格换行


\usepackage{hyperref}
\hypersetup{
    colorlinks=true,     % 启用颜色链接
    linkcolor=blue,     % 内部链接的颜色
    citecolor=blue,      % 引用文献的颜色
    urlcolor=blue,       % URL链接的颜色
    linktoc=red,      % 不影响目录链接颜色
}

\usepackage[a4paper, top=1in, bottom=1in, left=1in, right=1in]{geometry}

\title{
{\bf \huge Notes on M\"untz-Jackson Theorem}
%{\bf \large For M\"untz systems on [0,1]}
}
\author{Huaijin Wang}
\date{December 10, 2024}


\begin{document}


\newtheorem{definition}{Definition}[section]
\newtheorem{property}{Property}[section]
\newtheorem{lemma}{Lemma}[section]
\newtheorem{theorem}{Theorem}[section]
\newtheorem{corollary}{Corollary}[section]
\newtheorem{remark}{Remark}[section]
\newtheorem{example}{Example}[]
\newtheorem{notation}{Notation Declaration}[]
\newtheorem{question}{Question}[]
\newtheorem{exercise}{Exercise}[section]

%\maketitle




\newpage

\setcounter{section}{1}
\setcounter{exercise}{0}
\begin{exercise}
Let $A \in \mathbb{R}^{n\times n}$ be a symmetric positive define matrix, $b\in \mathbb{R}^n$. Prove that the following two problems have a same solution:
~\\
1. Find $x\in \mathbb{R}^n$ such that 
\begin{equation}
Ax=b.  \label{eq:1}
\end{equation}
~\\
2. Find $x\in \mathbb{R}^n$ such that 
\begin{equation}
J(x) =\min_{y\in \mathbb{R}^n} J(y),
\label{eq:2}
\end{equation}
 where $J(y) = \frac{1}{2} (Ax,x) - (x,b)$.
\end{exercise}
\begin{proof}
Suppose that $x$ is the solution of \eqref{eq:1}. Then for any $y\in\mathbb{R}^n$, we set $w = y-x$. Then it is clear that $(Ax, w) = (w,b)$, $(Aw,w) \geqslant 0$, and
\[
\begin{aligned}
J(y) & = J(w+x) = \frac{1}{2} (Aw+Ax, w+x) - (w+x,b) \\
& = \frac{1}{2} (Ax,x)-(x,b) + \frac{1}{2} (Aw, w) + (Ax,w)-(w,b) \\
& = J(x) + \frac{1}{2} (Aw,w) \geqslant J(x).
\end{aligned}
\]
Suppose that $x$ is the solution of \eqref{eq:2}. Then for any $y\in \mathbb{R}^n$ and $\alpha \in \mathbb{R}$, we have $J(x+\alpha y) \geqslant J(x)$, which is convex over $\alpha$ and attains its minimum at $\alpha=0$. Thus
\[
\frac{\mathrm{d} J(x+\alpha y)}{\mathrm{d} \alpha} \Big |_{\alpha=0} = 0,
\]
which leads to $(Ax-b, y) = 0$ giving rise to $Ax=b$.
\end{proof}




\end{document}

